ironfleet/src/Dafny/Distributed/Protocol/Raft/Types.i.dfy
@@ -13,13 +13,15 @@ type RaftPacket = LPacket<EndPoint, RaftMessage>
 type RaftIo = LIoOp<EndPoint, RaftMessage>
 
 datatype RaftMessage =
-    RequestVote(term:int, candidate_id:int, last_log_index:int, last_log_term:int)
-  | RequestVoteReply(term:int, vote_granted:bool)
-  | AppendEntries(term:int, leader_id:int, prev_log_index:int, prev_log_term:int, entries:seq<AppRequest>, leader_commit:int)
-  | AppendEntriesReply(term:int, success:bool)
+    RaftMessage_RequestVote(term:int, candidate_id:int, last_log_index:int, last_log_term:int)
+  | RaftMessage_RequestVoteReply(term:int, vote_granted:bool)
+  | RaftMessage_AppendEntries(term:int, leader_id:int, prev_log_index:int, prev_log_term:int, entries:seq<AppRequest>, leader_commit:int)
+  | RaftMessage_AppendEntriesReply(term:int, success:bool)
 
 datatype RaftRole = Follower | Candidate | Leader
 
 datatype ClockReading = ClockReading(t:int)
+
+datatype LogEntry = LogEntry(term:int, index:int, req:AppRequest)
 
 }
